coq/lib/Semantics/Reduce.v
@@ -22,25 +22,67 @@ where "'⟦' x ':=' v '⟧' e" := (sub x v e).
 Open Scope maybe_scope.
 Open Scope op_scope.
 
-(** Call-by-name Evaluation. *)
-Fixpoint rd (e : term) : option term :=
+Reserved Notation "e1 '-->'  e2"
+         (at level 70, no associativity).
+
+(** Call by name reduction. *)
+Inductive rd : term -> term -> Prop :=
+| rd_app_sub x e1 e2 :
+    (λ x ⇒ e1) ⋅ e2 -->  ⟦x:=e2⟧ e1
+| rd_app_l e1 e1' e2 :
+    e1 -->  e1' ->
+    e1 ⋅ e2 -->  e1' ⋅ e2
+| rd_cond_true e2 e3 :
+    Cond true e2 e3 -->  e2
+| rd_cond_false e2 e3 :
+    Cond false e2 e3 -->  e3
+| rd_cond_guard e1 e1' e2 e3 :
+    e1 -->  e1' ->
+    Cond e1 e2 e3 -->  Cond e1' e2 e3
+| rd_add (n1 n2 : nat) :
+    Op ⨥ n1 n2 -->  Nat (n1 + n2)
+| rd_sub (n1 n2 : nat) :
+    Op ⨪ n1 n2 -->  Nat (n1 - n2)
+| rd_eq (n1 n2 : nat) :
+    Op ≅ n1 n2 -->  Bool (n1 =? n2)
+| rd_lt (n1 n2 : nat) :
+    Op ⋖ n1 n2 -->  Bool (n1 <? n2)
+| rd_and (b1 b2 : bool) :
+    Op ∧ b1 b2 -->  Bool (b1 && b2)
+| rd_or (b1 b2 : bool) :
+    Op ∨ b1 b2 -->  Bool (b1 || b2)
+| rd_op_r_nat o (n : nat) e2 e2' :
+    e2 -->  e2' ->
+    Op o n e2 -->  Op o n e2'
+| rd_op_r_bool o (b : bool) e2 e2' :
+    e2 -->  e2' ->
+    Op o b e2 -->  Op o b e2'
+| rd_op_l o e1 e1' e2 :
+    e1 -->  e1' ->
+    Op o e1 e2 -->  Op o e1' e2
+| rd_let x e1 e2 :
+    LET x e1 e2 -->  ⟦x:=e1⟧ e2
+where "e1 '-->' e2" := (rd e1 e2) : type_scope.
+
+(** Call-by-name evaluation. *)
+Fixpoint eval (e : term) : option term :=
   match e with
   | Var _ | λ _ ⇒ _ | Bool _ | Nat _ => None
   | (λ x ⇒ e1) ⋅ e2 => Some (⟦x:=e2⟧ e1)
-  | e1 ⋅ e2 => let! e1' := rd e1 in e1' ⋅ e2
+  | e1 ⋅ e2 => let! e1' := eval e1 in e1' ⋅ e2
   | Cond true  e2 _ => Some e2
   | Cond false _ e3 => Some e3
-  | Cond e1 e2 e3 => let! e1' := rd e1 in Cond e1' e2 e3
+  | Cond e1 e2 e3 => let! e1' := eval e1 in Cond e1' e2 e3
   | LET x e1 e2 => Some (⟦x:=e1⟧ e2)
   | Op ⨥ (Nat n1)  (Nat n2)  => Some (Nat  (n1 + n2))
   | Op ⨪ (Nat n1)  (Nat n2)  => Some (Nat  (n1 - n2))
   | Op ∧ (Bool b1) (Bool b2) => Some (Bool (b1 &&  b2))
   | Op ∨ (Bool b1) (Bool b2) => Some (Bool (b1 || b2))
   | Op ≅ (Nat n1)  (Nat n2)  => Some (Bool (n1 =? n2))
-  | Op ≦ (Nat n1)  (Nat n2)  => Some (Bool (n1 <=? n2))
+  | Op ⋖ (Nat n1)  (Nat n2)  => Some (Bool (n1 <? n2))
   | Op o ((Nat _ | Bool _) as e1) e2 =>
-    let! e2' := rd e2 in Op o e1 e2'
-  | Op o e1 e2 => let! e1' := rd e1 in Op o e1' e2
+    let! e2' := eval e2 in Op o e1 e2'
+  | Op o e1 e2 => let! e1' := eval e1 in Op o e1' e2
   end.
 
 Inductive value : term -> Prop :=
