coq/lib/Semantics/Properties.v
@@ -24,16 +24,10 @@ End Canon.
 
 Section Progress.
   Local Hint Constructors value : core.
-  Local Hint Constructors typing : core.
-
-  Local Hint Extern 0 =>
-  match goal with
-  | |- context [if ?b then _ else _] =>
-    destruct b eqn:?; simpl
-  end : core.
+  Local Hint Constructors rd : core.
 
   Theorem prog : forall e t,
-      ∅ ⊨ e ∴ t -> value e \/ exists e', rd e = Some e'.
+      ∅ ⊨ e ∴ t -> value e \/ exists e', e -->  e'.
   Proof.
     intro e;
       induction e as
@@ -58,18 +52,10 @@ Section Progress.
                | H: ∅ ⊨ ?v ∴ TBool, Hv: value ?v
                  |- _ => pose proof canon_bool v Hv H as (? & ?);
                          clear Hv; subst; simpl
-               | H: rd ?e = Some _ |- context [rd ?e] => rewrite H; clear H
                | H: bound _ _ ∅ |- _ => unfold bound, "∅" in H; discriminate
-               end;
-        maybe_simpl; eauto;
-          try (destruct e1; eauto; assumption);
-          try (destruct e2; eauto; assumption);
-          try (destruct e1; destruct e2; eauto; assumption);
-          try (destruct e1; eauto;
-               match goal with
-               | H: _ ⊨ Nat _ ∴ TBool |- _ => inv H
-               | H: _ ⊨ Bool _ ∴ TNat |- _ => inv H
-               end; contradiction).
+               | H: _ ⊨ Bool ?b ∴ TBool
+                 |- context [Cond (Bool ?b) _ _ -->  _] => destruct b; clear H
+               end; eauto.
   Qed.
 End Progress.
 
@@ -128,5 +114,92 @@ Section Sub.
 End Sub.
 
 Section Preservation.
-  (* TODO *)
+  Local Hint Constructors typing : core.
+  Local Hint Constructors op_typs : core.
+  Local Hint Resolve sub_lemma : core.
+
+  Theorem preservation : forall e e',
+      e -->  e' -> forall t, ∅ ⊨ e ∴ t -> ∅ ⊨ e' ∴ t.
+  Proof.
+    intros e e' Hee'; induction Hee'; intros t Ht; inv Ht;
+      repeat match goal with
+             | H: op_typs _ _ _ |- _ => inv H
+             | H: _ ⊨ λ _ ⇒ _ ∴ _ |- _ => inv H
+             | H: _ ⊨ Bool _ ∴ TNat |- _ => inv H
+             | H: _ ⊨ Nat _ ∴ TBool |- _ => inv H
+             end; eauto.
+  Qed.
 End Preservation.
+
+Section EvalRd.
+  Lemma eval_complete : forall e e',
+    e -->  e' -> eval e = Some e'.
+  Proof.
+    intros e e' Hee'; induction Hee'; maybe_simpl; eauto.
+    - rewrite IHHee'. destruct e1; eauto. inv Hee'.
+    - rewrite IHHee'. destruct e1; eauto. inv Hee'.
+    - rewrite IHHee'.
+      destruct o; maybe_simpl; eauto;
+        destruct e2; eauto; inv Hee'.
+    - rewrite IHHee'.
+      destruct o; maybe_simpl; eauto;
+        destruct e2; eauto; inv Hee'.
+    - rewrite IHHee'.
+      destruct o; destruct e1;
+        maybe_simpl; eauto;
+          destruct e2; eauto; inv Hee'.
+  Qed.
+
+  Local Hint Constructors rd : core.
+
+  Ltac unwind :=
+    match goal with
+    | H: match eval ?e with
+         | Some _ => Some _
+         | None   => None
+         end = Some _ |- _ =>
+      assert (exists e', eval e = Some e')
+        by (destruct (eval e) as [? |] eqn:? ;
+            try discriminate; eauto);
+      match goal with
+      | Hex: (exists e', eval ?e = Some e') |- _ =>
+        destruct Hex as [? ?];
+        match goal with
+        | Heq: eval ?e = Some ?e' |- _ =>
+          rewrite Heq in H
+        end
+      end
+    end.
+  
+  Lemma eval_sound : forall e e',
+      eval e = Some e' -> e -->  e'.
+  Proof.
+    intro e;
+      induction e as
+        [ x
+        | x e IHe
+        | e1 IHe1 e2 IHe2
+        | n | b
+        | e1 IHe1 e2 IHe2 e3 IHe3
+        | o e1 IHe1 e2 IHe2
+        | x e1 IHe1 e2 IHe2 ];
+      intros e' Heval; simpl in *;
+        maybe_simpl_hyp Heval; try discriminate.
+    - destruct e1;
+        maybe_simpl_hyp Heval;
+        try discriminate;
+        try unwind; inv Heval; eauto.
+    - destruct e1;
+        maybe_simpl_hyp Heval;
+        try discriminate;
+        try unwind; inv Heval; eauto.
+      destruct b; inv H0; eauto.
+    - destruct o; destruct e1;
+        maybe_simpl_hyp Heval;
+        try discriminate;
+        try unwind; try (inv Heval; eauto; assumption);
+          destruct e2; try discriminate;
+            try unwind; inv Heval; eauto.
+    - inv Heval; eauto.
+  Qed.
+End EvalRd.
